chkpt evidence

src/program_proof/pav/evidence.v
@@ -13,10 +13,34 @@ Record t :=
     data: list w8;
   }.
 
-Definition encodesF (o : t) : list w8 :=
-  [(W8 1)] ++ u64_le o.(epoch) ++ o.(prevLink) ++ o.(data).
-Definition encodes (b : list w8) (o : t) : Prop :=
-  b = encodesF o.
+Definition encodesF (obj : t) : list w8 :=
+  [(W8 1)] ++ u64_le obj.(epoch) ++ obj.(prevLink) ++ obj.(data).
+Definition encodes (enc : list w8) (obj : t) : Prop :=
+  enc = encodesF obj.
+
+Section local_defs.
+Context `{!heapGS Σ}.
+Definition own ptr obj : iProp Σ :=
+  ∃ sl_prevLink sl_data,
+  "Hepoch" ∷ ptr ↦[chainSepSome :: "epoch"] #obj.(epoch) ∗
+  "HprevLink" ∷ ptr ↦[chainSepSome :: "prevLink"] (slice_val sl_prevLink) ∗
+  "Hsl_prevLink" ∷ own_slice_small sl_prevLink byteT (DfracOwn 1) obj.(prevLink) ∗
+  "Hdata" ∷ ptr ↦[chainSepSome :: "data"] (slice_val sl_data) ∗
+  "Hsl_data" ∷ own_slice_small sl_data byteT (DfracOwn 1) obj.(data).
+
+Lemma wp_encode ptr obj :
+  {{{
+    "Hobj" ∷ own ptr obj
+  }}}
+    chainSepSome__encode #ptr
+  {{{
+    sl_enc enc, RET (slice_val sl_enc);
+    "Hobj" ∷ own ptr obj ∗
+    "Hsl_enc" ∷ own_slice_small sl_enc byteT (DfracOwn 1) enc ∗
+    "%Henc" ∷ ⌜encodes enc obj⌝
+  }}}.
+Proof. Admitted.
+End local_defs.
 End chainSepSome.
 
 Module servSepLink.
@@ -25,10 +49,31 @@ Record t :=
     link: list w8;
   }.
 
-Definition encodesF (o : t) : list w8 :=
-  [(W8 0)] ++ o.(link).
-Definition encodes (b : list w8) (o : t) : Prop :=
-  b = encodesF o.
+Definition encodesF (obj : t) : list w8 :=
+  [(W8 0)] ++ obj.(link).
+Definition encodes (enc : list w8) (obj : t) : Prop :=
+  enc = encodesF obj.
+
+Section local_defs.
+Context `{!heapGS Σ}.
+Definition own ptr obj : iProp Σ :=
+  ∃ sl_link,
+  "Hlink" ∷ ptr ↦[servSepLink :: "link"] (slice_val sl_link) ∗
+  "Hsl_link" ∷ own_slice_small sl_link byteT (DfracOwn 1) obj.(link).
+
+Lemma wp_encode ptr obj :
+  {{{
+    "Hobj" ∷ own ptr obj
+  }}}
+    servSepLink__encode #ptr
+  {{{
+    sl_enc enc, RET (slice_val sl_enc);
+    "Hobj" ∷ own ptr obj ∗
+    "Hsl_enc" ∷ own_slice_small sl_enc byteT (DfracOwn 1) enc ∗
+    "%Henc" ∷ ⌜encodes enc obj⌝
+  }}}.
+Proof. Admitted.
+End local_defs.
 End servSepLink.
 
 Module servSepPut.
@@ -39,11 +84,47 @@ Record t :=
     val: list w8;
   }.
 
-Definition encodesF (o : t) : list w8 :=
-  [(W8 1)] ++ u64_le o.(epoch) ++ o.(id) ++ o.(val).
-Definition encodes (b : list w8) (o : t) : Prop :=
-  b = encodesF o.
+Definition encodesF (obj : t) : list w8 :=
+  [(W8 1)] ++ u64_le obj.(epoch) ++ obj.(id) ++ obj.(val).
+Definition encodes (enc : list w8) (obj : t) : Prop :=
+  enc = encodesF obj.
 End servSepPut.
+
+Module evidServLink.
+Record t :=
+  mk {
+    epoch0: w64;
+    prevLink0: list w8;
+    dig0: list w8;
+    sig0: list w8;
+
+    epoch1: w64;
+    prevLink1: list w8;
+    dig1: list w8;
+    sig1: list w8;
+  }.
+
+Section local_defs.
+Context `{!heapGS Σ}.
+Definition own ptr obj : iProp Σ :=
+  ∃ sl_prevLink0 sl_dig0 sl_sig0 sl_prevLink1 sl_dig1 sl_sig1,
+  "Hepoch0" ∷ ptr ↦[evidServLink :: "epoch0"] #obj.(epoch0) ∗
+  "HprevLink0" ∷ ptr ↦[evidServLink :: "prevLink0"] (slice_val sl_prevLink0) ∗
+  "Hsl_prevLink0" ∷ own_slice_small sl_prevLink0 byteT (DfracOwn 1) obj.(prevLink0) ∗
+  "Hdig0" ∷ ptr ↦[evidServLink :: "dig0"] (slice_val sl_dig0) ∗
+  "Hsl_dig0" ∷ own_slice_small sl_dig0 byteT (DfracOwn 1) obj.(dig0) ∗
+  "Hsig0" ∷ ptr ↦[evidServLink :: "sig0"] (slice_val sl_sig0) ∗
+  "Hsl_sig0" ∷ own_slice_small sl_sig0 byteT (DfracOwn 1) obj.(sig0) ∗
+
+  "Hepoch1" ∷ ptr ↦[evidServLink :: "epoch1"] #obj.(epoch1) ∗
+  "HprevLink1" ∷ ptr ↦[evidServLink :: "prevLink1"] (slice_val sl_prevLink1) ∗
+  "Hsl_prevLink1" ∷ own_slice_small sl_prevLink1 byteT (DfracOwn 1) obj.(prevLink1) ∗
+  "Hdig1" ∷ ptr ↦[evidServLink :: "dig1"] (slice_val sl_dig1) ∗
+  "Hsl_dig1" ∷ own_slice_small sl_dig1 byteT (DfracOwn 1) obj.(dig1) ∗
+  "Hsig1" ∷ ptr ↦[evidServLink :: "sig1"] (slice_val sl_sig1) ∗
+  "Hsl_sig1" ∷ own_slice_small sl_sig1 byteT (DfracOwn 1) obj.(sig1).
+End local_defs.
+End evidServLink.
 
 Section evidence.
 Context `{!heapGS Σ, !mono_listG (list w8) Σ}.
@@ -72,4 +153,64 @@ Definition serv_sigpred γ : (list w8 → iProp Σ) :=
         serv_sigpred_put γ dataSepPut
     )%I)%I.
 
+Lemma wp_evidServLink_check ptr_evid evid pk γ hon :
+  {{{
+    "Hevid" ∷ evidServLink.own ptr_evid evid ∗
+    "#Hpk" ∷ is_pk pk (serv_sigpred γ) hon
+  }}}
+  evidServLink__check #ptr_evid (slice_val pk)
+  {{{
+    (err : bool), RET #err;
+    "Hevid" ∷ evidServLink.own ptr_evid evid ∗
+    if negb err then
+      "%Hhon" ∷ ⌜hon = false⌝
+    else True%I
+  }}}.
+Proof.
+  rewrite /evidServLink__check.
+  iIntros (Φ) "H HΦ"; iNamed "H".
+  iDestruct "Hevid" as (??????) "H"; iNamed "H".
+  wp_loadField.
+  wp_loadField.
+  wp_loadField.
+  wp_apply wp_allocStruct; [val_ty|];
+    iIntros (ptr_linkSep0) "Hptr_linkSep0".
+  iDestruct (struct_fields_split with "Hptr_linkSep0") as "H";
+    iNamed "H"; iClear "tag".
+  wp_apply (chainSepSome.wp_encode with "[epoch prevLink data Hsl_prevLink0 Hsl_dig0]").
+  {
+    instantiate (1:=chainSepSome.mk _ _ _).
+    rewrite /chainSepSome.own /=.
+    iExists sl_prevLink0; iFrame.
+  }
+  iIntros (sl_link0Enc link0Enc) "H"; iNamed "H";
+    iRename "Hobj" into "Hptr_linkSep0";
+    iRename "Hsl_enc" into "Hsl_link0Enc";
+    rename Henc into Henc_link0.
+  wp_apply (wp_Hash with "Hsl_link0Enc");
+    iIntros (sl_link0 link0) "H"; iNamed "H";
+    iRename "Hdata" into "Hsl_link0Enc";
+    iRename "Hhash" into "Hsl_link0";
+    iRename "His_hash" into "His_hash_link0".
+  wp_apply wp_allocStruct; [val_ty|];
+    iIntros (ptr_enc0) "Hptr_enc0".
+  iDestruct (struct_fields_split with "Hptr_enc0") as "H";
+    iNamed "H"; iClear "tag".
+  wp_apply (servSepLink.wp_encode with "[link Hsl_link0]").
+  {
+    instantiate (1:=servSepLink.mk _).
+    rewrite /servSepLink.own /=.
+    iFrame.
+  }
+  iIntros (sl_enc0 enc0) "H"; iNamed "H";
+    iRename "Hobj" into "Hptr_enc0";
+    iRename "Hsl_enc" into "Hsl_enc0";
+    rename Henc into Henc_enc0.
+  wp_loadField.
+  wp_apply (wp_Verify with "[Hsl_enc0 Hsl_sig0]"); [iFrame "#∗"|];
+    iIntros (?) "H"; iNamed "H";
+    iRename "Hsig" into "Hsl_sig0";
+    iRename "Hmsg" into "Hsl_enc0".
+  destruct ok.
+Admitted.
 End evidence.
